Ghost task queue proven

share/steel/examples/pulse/parallel/GhostTaskQueue.fst
@@ -2,6 +2,7 @@ module GhostTaskQueue
 module L = FStar.List.Tot.Base
 module P = FStar.Preorder
 
+
 let smaller_status: P.preorder task_status =
 fun (x y: task_status) -> 
     match x, y with
@@ -56,6 +57,8 @@ Lemma (requires is_mono_suffix' x y /\ is_mono_suffix' y z)
     else is_same_trans x y z
   )
 
+val is_mono_suffix (#a: Type): P.preorder (mono_list a)
+
 let is_mono_suffix #a =
   introduce forall x. (is_mono_suffix' #a x x) with (is_mono_suffix_refl #a x);
   introduce forall x y z. (is_mono_suffix' #a x y /\ is_mono_suffix' y z
@@ -65,6 +68,8 @@ let is_mono_suffix #a =
     with _. (is_mono_suffix_trans x y z)
   );
   is_mono_suffix'
+
+val task_in_queue (#a: Type) (x: a) (pos:nat) (l: mono_list a): prop
 
 let rec task_in_queue #a (x: a) (pos:nat) (l: mono_list a) =
   if pos + 1 = L.length l then
@@ -102,6 +107,14 @@ pos:nat{task_in_queue t pos r})
 let enqueue_preserves_order l t:
 Lemma (is_mono_suffix l (enqueue_todo l t)._1)
 = is_same_refl l
+
+let rec count_ongoing #a (l: mono_list a): nat =
+match l with
+| [] -> 0
+| (_, s)::q -> (if s = Ongoing then 1 else 0) + count_ongoing q
+
+let get_actual_queue #a (l: mono_list a): list a =
+    L.map fst (L.filter (fun t -> Todo? (snd t)) l)
 
 // 2. pop: when a worker starts working on a task
 // it updates the task to "ongoing"
@@ -176,6 +189,24 @@ let ghost_mono_ref a = M.ref (mono_list a) is_mono_suffix
 let pts_to_ghost_queue #a (r: ghost_mono_ref a) (l: mono_list a): vprop
 = M.pts_to r full_perm l
 
+//open Pulse.Lib.Pervasives
+
+let pts_to_ghost_queue_half #a (r: ghost_mono_ref a) (l: mono_list a): vprop
+= M.pts_to r one_half l
+
+assume val share_queue_general #a (r: ghost_mono_ref a) (l: mono_list a) f:
+stt_ghost unit emp_inames (M.pts_to r f l)
+  (fun () -> M.pts_to r (half_perm f) l ** M.pts_to r (half_perm f) l)
+
+// TODO
+assume val share_queue #a (r: ghost_mono_ref a) (l: mono_list a):
+stt_ghost unit emp_inames (pts_to_ghost_queue r l)
+  (fun () -> pts_to_ghost_queue_half r l ** pts_to_ghost_queue_half r l)
+
+assume val gather_queue #a (r: ghost_mono_ref a) (l1: mono_list a) (l2: mono_list a):
+stt_ghost unit emp_inames (pts_to_ghost_queue_half r l1 ** pts_to_ghost_queue_half r l2)
+  (fun () -> pts_to_ghost_queue r l1 ** pure (l1 == l2))
+
 let alloc_ghost_queue (#a:Type)
   : stt_ghost (ghost_mono_ref a) emp_inames emp (fun r -> pts_to_ghost_queue r [])
 = M.alloc is_mono_suffix []
@@ -210,9 +241,20 @@ let recall (#a:Type u#1) #t #pos
            (w:M.witnessed r (task_in_queue t pos))
   : //TODO: SteelAtomicU
  stt_ghost unit emp_inames
+                 (pts_to_ghost_queue_half r v)
+                 (fun _ -> pts_to_ghost_queue_half r v ** pure (task_in_queue t pos v))
+  = M.recall (task_in_queue t pos) r v w
+
+let recall_full (#a:Type u#1) #t #pos
+           (r:ghost_mono_ref a)
+           (v:erased (mono_list a))
+           (w:M.witnessed r (task_in_queue t pos))
+  : //TODO: SteelAtomicU
+ stt_ghost unit emp_inames
                  (pts_to_ghost_queue r v)
                  (fun _ -> pts_to_ghost_queue r v ** pure (task_in_queue t pos v))
   = M.recall (task_in_queue t pos) r v w
+
 
 
 (** Part 3: Associated permissions: Reasoning done here **)
@@ -238,149 +280,195 @@ let get_certificate (t: task_elem) (pos: nat)
                   (fun _ -> pts_to_ghost_queue r l)
 = witness r l _
 
-let pts_to_Some (t: task_elem & task_status): vprop
-= (exists_ (fun v -> pts_to (t._1._2) #three_quart v ** pure (Some? v)))
+let pts_to_Some (t: task_elem & task_status) (f: perm): vprop
+= (exists_ (fun v -> pts_to (t._1._2) #f v ** pure (Some? v)))
 
+//let pts_to_Some (t: task_elem & task_status): vprop
+//= (exists_ (fun v -> pts_to (t._1._2) #three_quart v ** pure (Some? v)))
+
+
+
+let task_res_own (t: task_plus) (f: perm): vprop
+= match t._2 with
+| Todo -> pts_to (t._1._2) #f None
+| Ongoing -> emp // in this case, the worker has the half permission
+| Done -> pts_to_Some t f  //(exists_ (fun v -> pts_to (t._1._2) #three_quart v ** pure (Some? v)))
+
+(*
 let task_res_own (t: task_plus): vprop
 = match t._2 with
 | Todo -> pts_to (t._1._2) #three_quart None
 | Ongoing -> emp // in this case, the worker has the half permission
-| Done -> pts_to_Some t  //(exists_ (fun v -> pts_to (t._1._2) #three_quart v ** pure (Some? v)))
+| Done -> pts_to_Some t //(exists_ (fun v -> pts_to (t._1._2) #three_quart v ** pure (Some? v)))
+*)
 
+
+
+let rec tasks_res_own (l: mono_list_task_plus) (f: perm): vprop
+=  match l with
+  | [] -> emp
+  | tl::ql -> task_res_own tl f ** tasks_res_own ql f
   
+(*
 let rec tasks_res_own (l: mono_list_task_plus): vprop
 =  match l with
   | [] -> emp
   | tl::ql -> task_res_own tl ** tasks_res_own ql
+*)
 
 ```pulse
 ghost
-fn fold_done_task (t: task_elem) (l:mono_list_task_plus)
-  requires pts_to t._2 #three_quart None ** tasks_res_own l
-  ensures tasks_res_own (enqueue_todo l t)._1
+fn fold_done_task (t: task_elem) (l:mono_list_task_plus) (f: perm)
+  requires pts_to t._2 #f None ** tasks_res_own l f
+  ensures tasks_res_own (enqueue_todo l t)._1 f
 {
-  rewrite (pts_to t._2 #three_quart None) as (task_res_own (t, Todo));
-  fold (task_res_own (t, Todo));
-  rewrite (task_res_own (t, Todo) ** tasks_res_own l)
+  rewrite (pts_to t._2 #f None) as (task_res_own (t, Todo) f);
+  fold (task_res_own (t, Todo) f);
+  rewrite (task_res_own (t, Todo) f ** tasks_res_own l f)
     as
-  (tasks_res_own (enqueue_todo l t)._1);
+  (tasks_res_own (enqueue_todo l t)._1 f);
   ()
 }
 ```
 
+(*
+Old version:
 let small_inv (r: ghost_mono_ref task_elem) (q: list task_elem) (c: int): vprop 
 = exists_ (fun l -> pts_to_ghost_queue r l **
   tasks_res_own l **
   pure (count_ongoing l = c /\ get_actual_queue l == q)
 )
+*)
+
+//let three_eight = half_perm three_quart
+
+// TODO: Implement
+(*
+assume val share_tasks_res_own_quart (p: mono_list_task_plus):
+stt_ghost unit emp_inames (tasks_res_own p three_quart)
+(fun () -> tasks_res_own p one_half ** tasks_res_own p one_quart)
+*)
+
+assume val share_tasks_res_own (p: mono_list_task_plus):
+stt_ghost unit emp_inames (tasks_res_own p three_quart)
+(fun () -> tasks_res_own p one_half ** tasks_res_own p one_quart)
+
+assume val share_tasks_res_own_general (p: mono_list_task_plus) (f: perm):
+stt_ghost unit emp_inames (tasks_res_own p f)
+(fun () -> tasks_res_own p (half_perm f) ** tasks_res_own p (half_perm f))
+
+assume val share_task_res_own t (f: perm):
+stt_ghost unit emp_inames (task_res_own t f)
+(fun () -> task_res_own t (half_perm f) ** task_res_own t (half_perm f))
+
+
+
+
+
+let deadline (r: ghost_mono_ref task_elem): vprop
+= exists_ (fun f1 ->
+  exists_ (fun f2 ->
+  exists_ (fun l ->
+    M.pts_to r f1 l ** tasks_res_own l f2
+    ** pure (count_ongoing l = 0 /\ get_actual_queue l == [])
+  )))
+
+```pulse
+ghost fn
+duplicate_deadline' (r: ghost_mono_ref task_elem)
+requires deadline r
+ensures deadline r ** deadline r
+{
+  unfold deadline r;
+  with f1 f2 l. assert (M.pts_to r f1 l ** tasks_res_own l f2
+  ** pure (count_ongoing l = 0 /\ get_actual_queue l == []));
+  share_queue_general r l f1;
+  share_tasks_res_own_general l f2;
+  fold deadline r;
+  fold deadline r;
+  ()
+}
+```
+
+let duplicate_deadline = duplicate_deadline'
+
+```pulse
+ghost fn
+obtain_deadline (r: ghost_mono_ref task_elem) (f: perm)
+requires (exists l. pts_to_ghost_queue_half r l ** tasks_res_own l f **
+      pure (count_ongoing l = 0 /\ get_actual_queue l == []))
+  ensures deadline r
+{
+  with l. assert (pts_to_ghost_queue_half r l **
+      pure (count_ongoing l = 0 /\ get_actual_queue l == []));
+  unfold pts_to_ghost_queue_half r l;
+  assert (M.pts_to r one_half l ** pure (count_ongoing l = 0 /\ get_actual_queue l == []));
+  fold deadline r;
+  ()
+}
+```
+
+let small_inv (r: ghost_mono_ref task_elem) (q: list task_elem) (c: int): vprop 
+= exists_ (fun l -> pts_to_ghost_queue_half r l **
+  tasks_res_own l one_half **
+  pure (count_ongoing l = c /\ get_actual_queue l == q)
+  ** (if c = 0 && L.length q = 0 then deadline r
+  else pts_to_ghost_queue_half r l ** tasks_res_own l one_quart)
+)
+
+```pulse
+ghost fn
+extract_deadline' (r: ghost_mono_ref task_elem)
+requires small_inv r [] 0
+ensures small_inv r [] 0 ** deadline r
+{
+  unfold small_inv r [] 0;
+  with l. assert (pts_to_ghost_queue_half r l);
+  rewrite `@(if (0<:nat) = 0 && L.length ([] <: list task_elem) = 0 then deadline r
+    else pts_to_ghost_queue_half r l ** tasks_res_own l one_quart)
+  as deadline r;
+  duplicate_deadline r;
+  rewrite deadline r 
+    as `@(if (0<:nat) = 0 && L.length ([] <: list task_elem) = 0 then deadline r
+    else pts_to_ghost_queue_half r l ** tasks_res_own l one_quart);
+  fold small_inv r [] 0;
+  ()
+}
+```
+
+let extract_deadline = extract_deadline'
+
+```pulse
+ghost
+fn unfold_small_inv
+(r: ghost_mono_ref task_elem) (q: list task_elem) (c: int)
+requires small_inv r q c ** pure (c > 0)
+ensures exists l. (pts_to_ghost_queue r l
+  ** tasks_res_own l three_quart
+  ** pure (c = count_ongoing l /\ q == get_actual_queue l) 
+)
+{
+  admit()
+}
+```
+
+```pulse
+ghost
+fn fold_small_inv
+(r: ghost_mono_ref task_elem) (q: list task_elem) (c: int)
+requires exists l. (pts_to_ghost_queue r l
+  ** tasks_res_own l three_quart
+  ** pure (c = count_ongoing l /\ q == get_actual_queue l)
+  ** pure (c > 0 \/ L.length q > 0)
+  )
+ensures small_inv r q c
+{
+  admit()
+}
+```
+
 
 #push-options "--print_universes --print_implicits"
-
-// 1: Enqueue
-```pulse
-ghost
-fn spawn_task_ghost'
-(r: ghost_mono_ref task_elem)
-(q: list task_elem) (c: int) (t: task_elem)
-  requires small_inv r q c ** pts_to t._2 #three_quart None 
-  returns w: erased (pos:nat & certificate r t pos)
-  ensures small_inv r (t::q) c
-{
-  unfold (small_inv r q c);
-  with vl. assert (pts_to_ghost_queue r vl);
-  assert (tasks_res_own vl);
-  assert (pure (count_ongoing vl = c /\ get_actual_queue vl == q));
-  let p = enqueue_todo #task_elem vl t;
-  let pos = p._2;
-  assert (pure (task_in_queue t pos p._1));
-  write_ghost_queue #task_elem #vl r p._1;
-  assert (pts_to_ghost_queue r p._1);
-  let w: certificate r t pos = get_certificate t pos r p._1 _;
-  fold_done_task t vl;
-  fold (small_inv r (t::q) c);
-  let res = hide (| pos, w |);
-  res
-}
-```
-
-let spawn_task_ghost = spawn_task_ghost'
-
-let rec vprop_equiv_test
-  (l: mono_list_task_plus{~(get_actual_queue l == [])})
-: vprop_equiv (tasks_res_own l)
-  (pts_to (pop_todo_task l)._1._2 #three_quart None
-  ** tasks_res_own (pop_todo_task l)._2)
-= match l with
-| (t, Todo)::q ->
-let p1: vprop_equiv (tasks_res_own l) 
-  (pts_to (pop_todo_task l)._1._2 #three_quart None ** tasks_res_own q) = vprop_equiv_refl _ in
-let p2: vprop_equiv (tasks_res_own q) (emp ** tasks_res_own q) = 
-  vprop_equiv_sym _ _ (vprop_equiv_unit _)
- in
-let p3: vprop_equiv (emp ** tasks_res_own q) (tasks_res_own (pop_todo_task l)._2) = vprop_equiv_refl _ in
-let p4: vprop_equiv (tasks_res_own q) (tasks_res_own (pop_todo_task l)._2) = vprop_equiv_trans _ _ _ p2 p3 in
-let p5 = vprop_equiv_cong _ _ _ _ (vprop_equiv_refl (pts_to (pop_todo_task l)._1._2 #three_quart None)) p4 in
-vprop_equiv_trans _ _ _ p1 p5
-| t::q -> 
-let p1 = tasks_res_own l in
-let p2 = task_res_own t in
-let p3 = tasks_res_own q in
-let p4 = pts_to (pop_todo_task q)._1._2 #three_quart None in
-let p5 = tasks_res_own (pop_todo_task q)._2 in
-let p6 = tasks_res_own (pop_todo_task l)._2 in
-let e2: vprop_equiv p3 (p4 ** p5) = vprop_equiv_test q in
-let e3: vprop_equiv p1 (p2 ** (p4 ** p5)) = vprop_equiv_cong p2 p3 p2 (p4 ** p5) (vprop_equiv_refl _) e2 in
-let e4: vprop_equiv (p2 ** (p4 ** p5)) ((p2 ** p4) ** p5) = vprop_equiv_sym _ _ (vprop_equiv_assoc _ _ _) in
-let e5: vprop_equiv ((p2 ** p4) ** p5) ((p4 ** p2) ** p5) = vprop_equiv_cong (p2 ** p4) p5 (p4 ** p2) p5
-  (vprop_equiv_comm _ _) (vprop_equiv_refl _) in
-let e6: vprop_equiv ((p4 ** p2) ** p5) (p4 ** (p2 ** p5)) = vprop_equiv_assoc _ _ _ in
-let e7: vprop_equiv (p2 ** (p4 ** p5)) (p4 ** (p2 ** p5)) = vprop_equiv_trans _ _ _ e4 (vprop_equiv_trans _ _ _ e5 e6)
-in vprop_equiv_trans _ _ _ e3 e7
-
-let get_permission_from_todo
-  (l: mono_list_task_plus{~(get_actual_queue l == [])})
-: stt_ghost unit emp_inames
-(tasks_res_own l)
-  (fun _ -> pts_to (pop_todo_task l)._1._2 #three_quart None ** tasks_res_own (pop_todo_task l)._2)
-= rewrite _ _ (vprop_equiv_test l)
-
-let mk_erased_pair #r #t (pos: nat) (w: certificate r t pos):
-  erased (pos: nat & certificate r t pos)
-= hide (|pos, w|)
-  //returns pair:erased (pos:nat & certificate r t pos)
-
-// 2: Pop
-```pulse
-ghost
-fn pop_task_ghost'
-(r: ghost_mono_ref task_elem)
-(t: task_elem)
-(q: list task_elem) (c: int)
-  requires small_inv r (t::q) c
-  returns pair:erased (pos:nat & certificate r t pos)
-  ensures small_inv r q (c + 1) ** pts_to t._2 #three_quart None 
-{
-  unfold (small_inv r (t::q) c);
-  with l. assert (pts_to_ghost_queue r l);
-  assert (tasks_res_own l);
-  assert (pure (count_ongoing l = c /\ get_actual_queue l == t::q));
-  let p = pop_todo_task #task_elem l;
-  let order_is_preserved = pop_preserves_order #task_elem l;
-  write_ghost_queue #task_elem #l r p._2;
-  assert (pts_to_ghost_queue r p._2);
-  let certif: certificate r t p._3 = get_certificate t p._3 r p._2 ();
-  assert (pts_to_ghost_queue r p._2);
-  assert (pure (p._1 == t));
-  get_permission_from_todo l;
-  fold (small_inv r q (c + 1));
-  rewrite (pts_to (pop_todo_task l)._1._2 #three_quart None)
-    as (pts_to t._2 #three_quart None);
-  let pair: erased (pos:nat & certificate r t pos) = mk_erased_pair p._3 certif;//(| p._3, certif |);
-  pair
-}
-```
-
-let pop_task_ghost = pop_task_ghost'
 
 assume val pts_to_perm (#a: _) (#p: _) (#v: _) (r: ref a)
   : stt_ghost unit emp_inames
@@ -399,24 +487,327 @@ assume val share_pt
     (pts_to r #p v)
     (fun _ -> pts_to r #(half_perm p) v ** pts_to r #(half_perm p) v)
 
+let hperm = (f:perm{lesser_equal_perm one_half f})
+
 ```pulse
 ghost
 fn derive_false_from_too_much_permission
-(#a: Type) (r: ref a) (v1 v2: a)
-requires pts_to r #three_quart v1 ** pts_to r #three_quart v2
-ensures pts_to r #three_quart v1 ** pts_to r #three_quart v2
+(#a: Type) (r: ref a) (v1 v2: a) (f: hperm)
+requires pts_to r #f v1 ** pts_to r #three_quart v2
+ensures pts_to r #f v1 ** pts_to r #three_quart v2
   ** pure (~(r == r))
 {
-  gather_pt #a #three_quart #three_quart #v1 #v2 r;
-  pts_to_perm #_ #(sum_perm three_quart three_quart) #v1 r;
+  gather_pt #a #f #three_quart #v1 #v2 r;
+  pts_to_perm #_ #(sum_perm f three_quart) #v1 r;
   assert (pure False);
-  share_pt #a #(sum_perm three_quart three_quart) #v1 r;
-  rewrite (pts_to r #(half_perm (sum_perm three_quart three_quart)) v1 **
-    pts_to r #(half_perm (sum_perm three_quart three_quart)) v1)
-  as (pts_to r #three_quart v1 ** pts_to r #three_quart v2);
+  share_pt #a #(sum_perm f three_quart) #v1 r;
+  rewrite (pts_to r #(half_perm (sum_perm f three_quart)) v1 **
+    pts_to r #(half_perm (sum_perm f three_quart)) v1)
+  as (pts_to r #f v1 ** pts_to r #three_quart v2);
   ()
 }
 ```
+
+```pulse
+ghost
+fn derive_status_ongoing (h: (task_elem & task_status)) (x: option h._1._1) (f: hperm)
+  requires task_res_own h f ** (pts_to (h._1._2) #three_quart x)
+  ensures task_res_own h f ** (pts_to (h._1._2) #three_quart x) ** pure (h._2 = Ongoing)
+{
+  if (snd h = Todo) {
+    rewrite (task_res_own h f) as (pts_to (h._1._2) #f None);
+    derive_false_from_too_much_permission h._1._2 None x f;
+    assert (pure (h._2 = Ongoing));
+    rewrite (pts_to (h._1._2) #f None) as (task_res_own h f);
+    ()
+  }
+  else {
+    if (snd h = Done) {
+      rewrite (task_res_own h f) as (pts_to_Some h f);
+      unfold (pts_to_Some h f);
+      assert (exists_ (fun v -> pts_to (h._1._2) #f v ** pure (Some? v)));
+      with v. assert (pts_to (h._1._2) #f v ** pure (Some? v));
+      derive_false_from_too_much_permission h._1._2 v x f;
+      fold (pts_to_Some h f);
+      rewrite (pts_to_Some h f) as (task_res_own h f);
+      ()
+    }
+    else {
+      ()
+    }
+  }
+}
+```
+
+
+
+// waiting to have recursion in Pulse
+assume val prove_task_ongoing_aux_cb
+  (t: task_elem)
+  (pos: nat)
+  (v: option t._1)
+  (l: (l:mono_list_task_plus{task_in_queue t pos l /\ L.length l >= 1}))
+  (f: hperm)
+:
+stt_ghost unit emp_inames
+(tasks_res_own l f ** pts_to t._2 #three_quart v)
+(fun () -> tasks_res_own l f  ** pts_to t._2 #three_quart v
+  ** pure (count_ongoing l > 0))
+
+```pulse
+ghost
+fn fold_tasks_res_own
+  (h: (task_elem & task_status)) (q: mono_list_task_plus)
+  (f: hperm)
+requires task_res_own h f ** tasks_res_own q f
+ensures tasks_res_own (h::q) f
+{
+  rewrite (task_res_own h f ** tasks_res_own q f) as (tasks_res_own (h::q) f);
+  ()
+}
+```
+
+
+
+```pulse
+ghost
+fn prove_task_ongoing_aux
+  (t: task_elem)
+  (pos: nat)
+  (v: option t._1)
+  (l: (l:mono_list_task_plus{task_in_queue t pos l /\ L.length l >= 1}))
+  (f: hperm)
+//stt_ghost unit emp_inames
+requires tasks_res_own l f ** pts_to t._2 #three_quart v
+ensures tasks_res_own l f ** pts_to t._2 #three_quart v ** pure (count_ongoing l > 0)
+{
+  let h = L.hd l;
+  let q = L.tl l;
+
+  unfold (tasks_res_own l f);
+  rewrite `@(
+  match l with
+    | [] -> emp
+    | tl::ql -> task_res_own tl f ** tasks_res_own ql f)
+  as (task_res_own h f ** tasks_res_own q f);
+  assert (pts_to t._2 #three_quart v);
+  assert (task_res_own h f ** tasks_res_own q f);
+
+  if (pos + 1 = L.length l)
+  {
+    rewrite (pts_to (t._2) #three_quart v) as (pts_to (h._1._2) #three_quart v);
+    derive_status_ongoing h v f;
+    assert (pure (count_ongoing l > 0));
+    rewrite (pts_to (h._1._2) #three_quart v) as (pts_to (t._2) #three_quart v);
+    assert (pts_to t._2 #three_quart v);
+    fold_tasks_res_own h q f;
+    fold tasks_res_own l f;
+    ()
+  }
+  else {
+    prove_task_ongoing_aux_cb t pos v q f;
+    rewrite (task_res_own h f ** tasks_res_own q f) as
+      `@(match l with
+        | [] -> emp
+        | tl::ql -> task_res_own tl f ** tasks_res_own ql f);
+    fold (tasks_res_own l f);
+   ()
+ }
+}
+```
+
+```pulse
+ghost
+fn prove_task_ongoing'
+  (#t: task_elem)
+  (#pos: nat)
+  (#v: option t._1)
+  (r:ghost_mono_ref task_elem)
+  (q: list task_elem) (c: int)
+  //(l: (l:mono_list task_elem{task_in_queue t pos l /\ L.length l >= 1})):
+  (w:certificate r t pos)
+//stt_ghost unit emp_inames
+requires small_inv r q c ** pts_to t._2 #three_quart v
+ensures small_inv r q c ** pts_to t._2 #three_quart v ** pure (c > 0)
+{
+  unfold small_inv r q c;
+  with l. assert (pts_to_ghost_queue_half r l);
+  let proof = recall #task_elem #t #pos r l w;
+  assert (pure (task_in_queue t pos l));
+  assert (pure (L.length l >= 1));
+  prove_task_ongoing_aux t pos v l one_half;
+  fold small_inv r q c;
+  ()
+}
+```
+//l
+
+(*
+  unfold is_active ct;
+  with v. assert (pts_to ct._1._2 #three_quart v);
+  prove_task_ongoing' #ct._1 #ct._2 #v r q c ct._3;
+  assert (pure (c > 0));
+  fold is_active ct;
+
+  unfold_small_inv r q c;
+
+*)
+
+// 1: Enqueue
+```pulse
+ghost
+fn spawn_task_ghost'
+(r: ghost_mono_ref task_elem)
+(q: list task_elem) (c: int) (t: task_elem)
+(ct: current_task r)
+  requires small_inv r q c ** pts_to t._2 #three_quart None ** is_active ct
+  returns w: erased (pos:nat & certificate r t pos)
+  ensures small_inv r (t::q) c ** is_active ct
+{
+  (*
+fn prove_task_ongoing'
+  (#t: task_elem)
+  (#pos: nat)
+  (#v: option t._1)
+  (r:ghost_mono_ref task_elem)
+  (q: list task_elem) (c: int)
+  //(l: (l:mono_list task_elem{task_in_queue t pos l /\ L.length l >= 1})):
+  (w:certificate r t pos)
+//stt_ghost unit emp_inames
+requires small_inv r q c ** pts_to t._2 #three_quart v
+ensures small_inv r q c ** pts_to t._2 #three_quart v ** pure (c > 0)
+{
+  *)
+
+  unfold is_active ct;
+  with v. assert (pts_to ct._1._2 #three_quart v);
+  prove_task_ongoing' #ct._1 #ct._2 #v r q c ct._3;
+  assert (pure (c > 0));
+  fold is_active ct;
+
+  unfold_small_inv r q c;
+  //unfold (small_inv r q c);
+
+
+  with vl. assert (pts_to_ghost_queue r vl);
+  assert (tasks_res_own vl three_quart);
+  assert (pure (count_ongoing vl = c /\ get_actual_queue vl == q));
+  let p = enqueue_todo #task_elem vl t;
+  let pos = p._2;
+  assert (pure (task_in_queue t pos p._1));
+  write_ghost_queue #task_elem #vl r p._1;
+  assert (pts_to_ghost_queue r p._1);
+  let w: certificate r t pos = get_certificate t pos r p._1 _;
+  assert (tasks_res_own vl three_quart);
+  fold_done_task t vl three_quart;
+  assert (tasks_res_own (enqueue_todo vl t)._1 three_quart);
+  assert (pts_to_ghost_queue r p._1);
+  rewrite (tasks_res_own (enqueue_todo vl t)._1 three_quart)
+    as (tasks_res_own p._1 three_quart);
+
+  fold_small_inv r (t::q) c;
+  //fold (small_inv r (t::q) c);
+  let res = hide (| pos, w |);
+  res
+}
+```
+
+let spawn_task_ghost = spawn_task_ghost'
+
+let rec vprop_equiv_test
+  (l: mono_list_task_plus{~(get_actual_queue l == [])}) (f: perm)
+: vprop_equiv (tasks_res_own l f)
+  (pts_to (pop_todo_task l)._1._2 #f None
+  ** tasks_res_own (pop_todo_task l)._2 f)
+= match l with
+| (t, Todo)::q ->
+let p1: vprop_equiv (tasks_res_own l f) 
+  (pts_to (pop_todo_task l)._1._2 #f None ** tasks_res_own q f) = vprop_equiv_refl _ in
+let p2: vprop_equiv (tasks_res_own q f) (emp ** tasks_res_own q f) = 
+  vprop_equiv_sym _ _ (vprop_equiv_unit _)
+ in
+let p3: vprop_equiv (emp ** tasks_res_own q f) (tasks_res_own (pop_todo_task l)._2 f) = vprop_equiv_refl _ in
+let p4: vprop_equiv (tasks_res_own q f) (tasks_res_own (pop_todo_task l)._2 f) = vprop_equiv_trans _ _ _ p2 p3 in
+let p5 = vprop_equiv_cong _ _ _ _ (vprop_equiv_refl (pts_to (pop_todo_task l)._1._2 #f None)) p4 in
+vprop_equiv_trans _ _ _ p1 p5
+| t::q -> 
+let p1 = tasks_res_own l f in
+let p2 = task_res_own t f in
+let p3 = tasks_res_own q f in
+let p4 = pts_to (pop_todo_task q)._1._2 #f None in
+let p5 = tasks_res_own (pop_todo_task q)._2 f in
+let p6 = tasks_res_own (pop_todo_task l)._2 f in
+let e2: vprop_equiv p3 (p4 ** p5) = vprop_equiv_test q f in
+let e3: vprop_equiv p1 (p2 ** (p4 ** p5)) = vprop_equiv_cong p2 p3 p2 (p4 ** p5) (vprop_equiv_refl _) e2 in
+let e4: vprop_equiv (p2 ** (p4 ** p5)) ((p2 ** p4) ** p5) = vprop_equiv_sym _ _ (vprop_equiv_assoc _ _ _) in
+let e5: vprop_equiv ((p2 ** p4) ** p5) ((p4 ** p2) ** p5) = vprop_equiv_cong (p2 ** p4) p5 (p4 ** p2) p5
+  (vprop_equiv_comm _ _) (vprop_equiv_refl _) in
+let e6: vprop_equiv ((p4 ** p2) ** p5) (p4 ** (p2 ** p5)) = vprop_equiv_assoc _ _ _ in
+let e7: vprop_equiv (p2 ** (p4 ** p5)) (p4 ** (p2 ** p5)) = vprop_equiv_trans _ _ _ e4 (vprop_equiv_trans _ _ _ e5 e6)
+in vprop_equiv_trans _ _ _ e3 e7
+
+let get_permission_from_todo
+  (l: mono_list_task_plus{~(get_actual_queue l == [])}) (f:perm)
+: stt_ghost unit emp_inames
+(tasks_res_own l f)
+  (fun _ -> pts_to (pop_todo_task l)._1._2 #f None ** tasks_res_own (pop_todo_task l)._2 f)
+= rewrite _ _ (vprop_equiv_test l f)
+
+let mk_erased_pair #r #t (pos: nat) (w: certificate r t pos):
+  erased (pos: nat & certificate r t pos)
+= hide (|pos, w|)
+  //returns pair:erased (pos:nat & certificate r t pos)
+
+// 2: Pop
+```pulse
+ghost
+fn pop_task_ghost'
+(r: ghost_mono_ref task_elem)
+(t: task_elem)
+(q: list task_elem) (c: int)
+(ct: current_task r)
+  requires small_inv r (t::q) c ** is_active ct
+  returns pair:erased (pos:nat & certificate r t pos)
+  ensures small_inv r q (c + 1) ** pts_to t._2 #three_quart None ** is_active ct
+{
+  unfold is_active ct;
+  with v. assert (pts_to ct._1._2 #three_quart v);
+  prove_task_ongoing' #ct._1 #ct._2 #v r (t::q) c ct._3;
+  assert (pure (c > 0));
+  fold is_active ct;
+  unfold_small_inv r (t::q) c;
+
+  //unfold (small_inv r (t::q) c);
+  with l. assert (pts_to_ghost_queue r l);
+  assert (tasks_res_own l three_quart);
+  assert (pure (count_ongoing l = c /\ get_actual_queue l == t::q));
+  let p = pop_todo_task #task_elem l;
+  let order_is_preserved = pop_preserves_order #task_elem l;
+  write_ghost_queue #task_elem #l r p._2;
+  assert (pts_to_ghost_queue r p._2);
+  let certif: certificate r t p._3 = get_certificate t p._3 r p._2 ();
+  assert (pts_to_ghost_queue r p._2);
+  assert (pure (p._1 == t));
+  get_permission_from_todo l three_quart;
+  (*
+requires exists l. (pts_to_ghost_queue r l
+  ** tasks_res_own l three_quart
+  ** pure (c = count_ongoing l /\ q == get_actual_queue l)
+  ** pure (c > 0)
+  )
+  *)
+  rewrite (tasks_res_own (pop_todo_task l)._2 three_quart)
+    as (tasks_res_own p._2 three_quart);
+  fold_small_inv r q (c + 1);
+  //fold (small_inv r q (c + 1));
+  rewrite (pts_to (pop_todo_task l)._1._2 #three_quart None)
+    as (pts_to t._2 #three_quart None);
+  let pair: erased (pos:nat & certificate r t pos) = mk_erased_pair p._3 certif;//(| p._3, certif |);
+  pair
+}
+```
+
+let pop_task_ghost = pop_task_ghost'
 
 let rec close_task_bis #a
     (t: a)
@@ -449,56 +840,14 @@ let close_task_bis_preserves_order #a
 
 ```pulse
 ghost
-fn derive_status_ongoing (h: (task_elem & task_status)) (x: option h._1._1)
-  requires task_res_own h ** (pts_to (h._1._2) #three_quart x)
-  ensures task_res_own h ** (pts_to (h._1._2) #three_quart x) ** pure (h._2 = Ongoing)
+fn fold_task_done (h:(task_elem & task_status)) (f: perm)
+  requires pts_to h._1._2 #f (Some x) ** pure (h._2 = Done)
+  ensures task_res_own h f
 {
-  if (snd h = Todo) {
-    rewrite (task_res_own h) as (pts_to (h._1._2) #three_quart None);
-    derive_false_from_too_much_permission h._1._2 None x;
-    assert (pure (h._2 = Ongoing));
-    rewrite (pts_to (h._1._2) #three_quart None) as (task_res_own h);
-    ()
-  }
-  else {
-    if (snd h = Done) {
-      rewrite (task_res_own h) as (pts_to_Some h);
-      unfold (pts_to_Some h);
-      assert (exists_ (fun v -> pts_to (h._1._2) #three_quart v ** pure (Some? v)));
-      with v. assert (pts_to (h._1._2) #three_quart v ** pure (Some? v));
-      derive_false_from_too_much_permission h._1._2 v x;
-      fold (pts_to_Some h);
-      rewrite (pts_to_Some h) as (task_res_own h);
-      ()
-    }
-    else {
-      ()
-    }
-  }
-}
-```
-
-```pulse
-ghost
-fn fold_task_done (h:(task_elem & task_status))
-  requires pts_to h._1._2 #three_quart (Some x) ** pure (h._2 = Done)
-  ensures task_res_own h
-{
-  assert (pts_to h._1._2 #three_quart (Some x) ** pure (Some? (Some x)));
-  intro_exists (fun v -> pts_to h._1._2 #three_quart v ** pure (Some? v)) (Some x);
-  rewrite (exists_ (fun v -> pts_to h._1._2 #three_quart v ** pure (Some? v))) as (pts_to_Some h);
-  rewrite (pts_to_Some h) as (task_res_own h);
-  ()
-}
-```
-
-```pulse
-ghost
-fn fold_tasks_res_own (h: (task_elem & task_status)) (q: mono_list_task_plus)
-requires task_res_own h ** tasks_res_own q
-ensures tasks_res_own (h::q)
-{
-  rewrite (task_res_own h ** tasks_res_own q) as (tasks_res_own (h::q));
+  assert (pts_to h._1._2 #f (Some x) ** pure (Some? (Some x)));
+  intro_exists (fun v -> pts_to h._1._2 #f v ** pure (Some? v)) (Some x);
+  rewrite (exists_ (fun v -> pts_to h._1._2 #f v ** pure (Some? v))) as (pts_to_Some h f);
+  rewrite (pts_to_Some h f) as (task_res_own h f);
   ()
 }
 ```
@@ -511,10 +860,38 @@ assume val put_back_permission_cb
   (x: t._1)
 :
 stt_ghost unit emp_inames
-(tasks_res_own l ** pts_to t._2 #three_quart (Some x))
-(fun () -> tasks_res_own (close_task_bis t pos l) ** pure (
+(tasks_res_own l three_quart ** pts_to t._2 #three_quart (Some x))
+(fun () -> tasks_res_own (close_task_bis t pos l) three_quart ** pure (
  get_actual_queue (close_task_bis t pos l) == get_actual_queue l
   /\ count_ongoing (close_task_bis t pos l) + 1 == count_ongoing l))
+
+// assuming because of universe polymorphism
+assume val
+stt_return #a (x:a): stt a emp (fun y -> pure (x == y))
+
+```pulse
+ghost
+fn fold_tasks_res_own_bis
+  (h: (task_elem & task_status)) 
+  (h': (task_elem & task_status))
+  (q: mono_list_task_plus)
+ (pos: nat) (t: task_elem)
+(l: (l:mono_list_task_plus{task_in_queue t pos l /\ b2t (L.length l >= 1)}))
+requires task_res_own h' three_quart ** tasks_res_own q three_quart
+  ** pure (t == h._1 /\ h == L.hd l /\ q == L.tl l /\ h' == (h._1, Done)
+  /\ pos + 1 = L.length l
+  )
+  //** pure (t == h._1 /\ h == L.hd l /\ q == L.tl l)
+//ensures tasks_res_own (h::q) f
+ensures tasks_res_own (close_task_bis u#1 #task_elem t pos l) three_quart
+{
+  rewrite (task_res_own h' three_quart ** tasks_res_own q three_quart) as (tasks_res_own (h'::q) three_quart);
+  rewrite (tasks_res_own (h'::q) three_quart)
+    as (tasks_res_own (close_task_bis u#1 #task_elem t pos l) three_quart);
+  ()
+}
+```
+
 
 
 
@@ -525,32 +902,32 @@ fn put_back_permission
   (pos: nat)
   (l: (l:mono_list_task_plus{task_in_queue t pos l /\ L.length l >= 1}))
   (x: t._1)
-requires tasks_res_own l ** pts_to t._2 #three_quart (Some x)
-ensures tasks_res_own (close_task_bis t pos l) ** pure (
+requires tasks_res_own l three_quart ** pts_to t._2 #three_quart (Some x)
+ensures tasks_res_own (close_task_bis t pos l) three_quart ** pure (
  get_actual_queue (close_task_bis t pos l) == get_actual_queue l
   /\ count_ongoing (close_task_bis t pos l) + 1 == count_ongoing l)
 {
   let h = L.hd l;
   let q = L.tl l;
 
-  unfold (tasks_res_own l);
+  unfold (tasks_res_own l three_quart);
   rewrite `@(
   match l with
     | [] -> emp
-    | tl::ql -> task_res_own tl ** tasks_res_own ql)
-  as (task_res_own h ** tasks_res_own q);
+    | tl::ql -> task_res_own tl three_quart ** tasks_res_own ql three_quart)
+  as (task_res_own h three_quart ** tasks_res_own q three_quart);
   assert (pts_to t._2 #three_quart (Some x));
-  assert (task_res_own h ** tasks_res_own q);
+  assert (task_res_own h three_quart ** tasks_res_own q three_quart);
 
   if (pos + 1 = L.length l)
   {
-    assert (task_res_own h);
+    assert (task_res_own h three_quart);
     rewrite (pts_to (t._2) #three_quart (Some x)) as (pts_to (h._1._2) #three_quart (Some x));
-    derive_status_ongoing h (Some x);
+    derive_status_ongoing h (Some x) three_quart;
     assert (pure (snd h = Ongoing));
     assert (pts_to (h._1._2) #three_quart (Some x));
 
-    unfold (task_res_own h); // not needed, can be dropped
+    unfold (task_res_own h three_quart); // not needed, can be dropped
     rewrite `@(match h._2 with
       | Todo -> pts_to (h._1._2) #three_quart None
       | Ongoing -> emp
@@ -559,111 +936,31 @@ ensures tasks_res_own (close_task_bis t pos l) ** pure (
 
     let h' = (h._1, Done);
     rewrite (pts_to (h._1._2) #three_quart (Some x)) as (pts_to h'._1._2 #three_quart (Some x));
-    fold_task_done h';
-    fold_tasks_res_own h' q;
+    fold_task_done h' three_quart;
+    fold_tasks_res_own_bis h h' q pos t l;
+    assert (tasks_res_own (close_task_bis u#1 #task_elem t pos l) three_quart);
     ()
+
   }
   else {
     put_back_permission_cb t pos q x;
-    assert (tasks_res_own (close_task_bis t pos q));
+    assert (tasks_res_own (close_task_bis t pos q) three_quart);
     assert (pure (get_actual_queue (close_task_bis t pos q) == get_actual_queue q));
     assert (pure (get_actual_queue (close_task_bis t pos l) == get_actual_queue l));
     assert (pure (count_ongoing (close_task_bis t pos q) + 1 == count_ongoing q));
     assert (pure (count_ongoing (close_task_bis t pos l) + 1 == count_ongoing l));
 
-    rewrite (task_res_own h ** tasks_res_own (close_task_bis t pos q)) as
+    rewrite (task_res_own h three_quart ** tasks_res_own (close_task_bis t pos q) three_quart) as
     `@(
     match (close_task_bis t pos l) with
       | [] -> emp
-      | tl::ql -> task_res_own tl ** tasks_res_own ql);
-    fold (tasks_res_own (close_task_bis t pos l));
+      | tl::ql -> task_res_own tl three_quart ** tasks_res_own ql three_quart);
+    fold (tasks_res_own (close_task_bis t pos l) three_quart);
     ()
   }
 }
 ```
 
-// waiting to have recursion in Pulse
-assume val prove_task_ongoing_aux_cb
-  (t: task_elem)
-  (pos: nat)
-  (v: option t._1)
-  (l: (l:mono_list_task_plus{task_in_queue t pos l /\ L.length l >= 1}))
-:
-stt_ghost unit emp_inames
-(tasks_res_own l ** pts_to t._2 #three_quart v)
-(fun () -> tasks_res_own l ** pts_to t._2 #three_quart v
-  ** pure (count_ongoing l > 0))
-// TODO: Implement this thing
-
-```pulse
-ghost
-fn prove_task_ongoing_aux
-  (t: task_elem)
-  (pos: nat)
-  (v: option t._1)
-  (l: (l:mono_list_task_plus{task_in_queue t pos l /\ L.length l >= 1}))
-//stt_ghost unit emp_inames
-requires tasks_res_own l ** pts_to t._2 #three_quart v
-ensures tasks_res_own l ** pts_to t._2 #three_quart v ** pure (count_ongoing l > 0)
-{
-  let h = L.hd l;
-  let q = L.tl l;
-
-  unfold (tasks_res_own l);
-  rewrite `@(
-  match l with
-    | [] -> emp
-    | tl::ql -> task_res_own tl ** tasks_res_own ql)
-  as (task_res_own h ** tasks_res_own q);
-  assert (pts_to t._2 #three_quart v);
-  assert (task_res_own h ** tasks_res_own q);
-
-  if (pos + 1 = L.length l)
-  {
-    rewrite (pts_to (t._2) #three_quart v) as (pts_to (h._1._2) #three_quart v);
-    derive_status_ongoing h v;
-    assert (pure (count_ongoing l > 0));
-    rewrite (pts_to (h._1._2) #three_quart v) as (pts_to (t._2) #three_quart v);
-    assert (pts_to t._2 #three_quart v);
-    fold_tasks_res_own h q;
-    ()
-  }
-  else {
-    prove_task_ongoing_aux_cb t pos v q;
-    rewrite (task_res_own h ** tasks_res_own q) as
-      `@(match l with
-        | [] -> emp
-        | tl::ql -> task_res_own tl ** tasks_res_own ql);
-    fold (tasks_res_own l);
-   ()
- }
-}
-```
-
-```pulse
-ghost
-fn prove_task_ongoing'
-  (#t: task_elem)
-  (#pos: nat)
-  (#v: option t._1)
-  (r:ghost_mono_ref task_elem)
-  (q: list task_elem) (c: int)
-  //(l: (l:mono_list task_elem{task_in_queue t pos l /\ L.length l >= 1})):
-  (w:certificate r t pos)
-//stt_ghost unit emp_inames
-requires small_inv r q c ** pts_to t._2 #three_quart v
-ensures small_inv r q c ** pts_to t._2 #three_quart v ** pure (c > 0)
-{
-  unfold small_inv r q c;
-  with l. assert (pts_to_ghost_queue r l);
-  let proof = recall #task_elem #t #pos r l w;
-  assert (pure (task_in_queue t pos l));
-  assert (pure (L.length l >= 1));
-  prove_task_ongoing_aux t pos v l;
-  fold small_inv r q c;
-  ()
-}
-```
 let prove_task_ongoing = prove_task_ongoing'
 
 ```pulse
@@ -680,7 +977,32 @@ ensures small_inv r q c ** pure (c >= 0)
 }
 ```
 
+// TODO
 let prove_ongoing_non_neg = prove_ongoing_non_neg'
+
+#push-options "--print_implicits --print_universes"
+
+assume val assume_prop (p: prop): stt_ghost unit emp_inames emp (fun () -> pure p)
+
+```pulse
+ghost fn imp_false (b: bool) (p: vprop)
+  requires pure (b == false)
+  ensures imp_vprop b p
+{
+  rewrite emp as (imp_vprop b p);
+  ()
+}
+```
+
+```pulse
+ghost fn imp_true (b: bool) (p: vprop)
+  requires pure (b == true) ** p
+  ensures imp_vprop b p
+{
+  rewrite p as (imp_vprop b p);
+  ()
+}
+```
 
 
 
@@ -695,20 +1017,58 @@ fn conclude_task_ghost'
 (x: t._1)
 (w: certificate r t pos)
   requires small_inv r q c ** pts_to t._2 #three_quart (Some x)
-  ensures small_inv r q (c - 1) 
+  ensures small_inv r q (c - 1) ** imp_vprop (c = 1 && L.length q = 0) (deadline r)
 {
-  unfold (small_inv r q c);
+  prove_task_ongoing' #t #pos #(Some x) r q c w;
+  assert (pure (c > 0));
+  unfold_small_inv r q c;
+  //unfold (small_inv r q c);
   with l. assert (pts_to_ghost_queue r l);
-  assert (tasks_res_own l);
+  assert (tasks_res_own l three_quart);
   assert (pure (count_ongoing l = c /\ get_actual_queue l == q));
-  let proof = recall #task_elem #t #pos r l w;
+  let proof = recall_full #task_elem #t #pos r l w;
   let p = close_task_bis t pos l;
   let order_is_preserved = close_task_bis_preserves_order #task_elem t pos l;
   write_ghost_queue #task_elem #l r p;
+  assert (pts_to_ghost_queue r p);
+
   put_back_permission t pos l x;
-  assert (tasks_res_own (close_task_bis t pos l));
-  fold (small_inv r q (c - 1));
-  ()
+  assert (tasks_res_own (close_task_bis t pos l) three_quart);
+
+  rewrite (tasks_res_own (close_task_bis u#1 #task_elem t pos (reveal u#1 #(mono_list u#1 task_elem) l)) three_quart)
+    as (tasks_res_own p three_quart);
+
+  assert (pts_to_ghost_queue r p);
+  assert (pure (c - 1 = count_ongoing p /\ q == get_actual_queue p));
+
+  let b: bool = stt_ghost_reveal _ (c - 1 = 0 && L.length q = 0);
+  if (b)
+  {
+    share_queue r p;
+    share_tasks_res_own p;
+    obtain_deadline r one_quart;
+    duplicate_deadline r;
+
+    assert (pts_to_ghost_queue_half r p);
+    //assert (tasks_res_own p one_half ** tasks_res_own p one_quart);
+    rewrite (deadline r)
+      as `@(if c - 1 = 0 && L.length q = 0 then deadline r
+      else pts_to_ghost_queue_half r l ** tasks_res_own l one_quart);
+
+    assert (pts_to_ghost_queue_half r p **
+      tasks_res_own p one_half **
+      pure (count_ongoing p = c - 1 /\ get_actual_queue p == q)
+      ** `@(if c - 1 = 0 && L.length q = 0 then deadline r
+      else pts_to_ghost_queue_half r p ** tasks_res_own p one_quart));
+    fold (small_inv r q (c - 1));
+    imp_true (c = 1 && L.length q = 0) (deadline r);
+    ()
+  }
+  else {
+    fold_small_inv r q (c - 1);
+    imp_false (c = 1 && L.length q = 0) (deadline r);
+    ()
+  }
 }
 ```
 
@@ -718,84 +1078,126 @@ let recall_certificate (#t: task_elem) (#pos: nat)
            (r:ghost_mono_ref task_elem)
            (v: mono_list task_elem)
            (w:certificate r t pos)
-= recall r v w
+= recall_full r v w
+
+assume val drop (p: vprop): stt_ghost unit emp_inames p (fun () -> emp)
+
+let pts_to_Some_fract (t:task_elem) (f: perm): vprop
+= (exists_ (fun v -> pts_to t._2 #f v ** pure (Some? v)))
 
 // assuming recursion
 assume val get_Some_finished_aux_rec
   (t: task_elem) (pos: nat)
   (l: mono_list_task_plus)
-: stt_ghost t._1 emp_inames
-(tasks_res_own l ** pure (task_in_queue t pos l) ** pure (count_ongoing l = 0 /\ get_actual_queue l == []))
-(fun _ -> tasks_res_own l)
+  (f: perm)
+: stt_ghost unit emp_inames
+(tasks_res_own l f ** pure (task_in_queue t pos l) ** pure (count_ongoing l = 0 /\ get_actual_queue l == []))
+(fun _ -> tasks_res_own l (half_perm f) ** pts_to_Some_fract t (half_perm f))
 
 ```pulse
 ghost
 fn get_Some_finished_aux
   (t: task_elem) (pos: nat)
   (l: mono_list_task_plus)
-requires tasks_res_own l ** pure (task_in_queue t pos l)
+  (f: perm)
+requires tasks_res_own l f ** pure (task_in_queue t pos l)
   ** pure (count_ongoing l = 0 /\ get_actual_queue l == [])
-returns x: t._1
-ensures tasks_res_own l
+//returns x: t._1
+//ensures tasks_res_own l f
+ensures tasks_res_own l (half_perm f) ** pts_to_Some_fract t (half_perm f)
 {
   let h = L.hd l;
   let q = L.tl l;
 
-  rewrite (tasks_res_own l) as (task_res_own h ** tasks_res_own q);
+  rewrite (tasks_res_own l f) as (task_res_own h f ** tasks_res_own q f);
 
   if (pos + 1 = L.length l)
   {
-    assert (task_res_own h);
+    assert (task_res_own h f);
     assert (pure (fst h == t));
     assert (pure (snd h = Done));
-    rewrite (task_res_own h) as (pts_to_Some h);
-    unfold (pts_to_Some h);
-    with y. assert (pts_to h._1._2 #three_quart y);
-    fold (pts_to_Some h);
-    rewrite (pts_to_Some h) as (task_res_own h);
-    rewrite (task_res_own h ** tasks_res_own q) as (tasks_res_own l);
-    let x = Some?.v y;
-    x
+    rewrite (task_res_own h f) as (pts_to_Some h f);
+    unfold (pts_to_Some h f);
+    with y. assert (pts_to h._1._2 #f y);
+    share #_ #emp_inames h._1._2;
+    //rewrite (pts_to_Some h (half_perm f)) as (pts_to_Some_fract t (half_perm f));
+    //fold (pts_to_Some h (half_perm f));
+    (*
+fn fold_task_done (h:(task_elem & task_status)) (f: perm)
+  requires pts_to h._1._2 #f (Some x) ** pure (h._2 = Done)
+  ensures task_res_own h f
+{
+  *)
+    with v. assert (pts_to h._1._2 #(half_perm f) v ** pure (Some? v));
+    //let x = Some?.v y;
+    assert (pure (Some (Some?.v v) == v));
+    rewrite (pts_to h._1._2 #(half_perm f) v) as (pts_to h._1._2 #(half_perm f) (Some (Some?.v v)));
+    rewrite (pts_to h._1._2 #(half_perm f) v) as (pts_to h._1._2 #(half_perm f) (Some (Some?.v v)));
+
+    //assert pts_to h._1._2 #f (Some x) ** pure (h._2 = Done)
+    fold_task_done h (half_perm f);
+    //fold (pts_to_Some_fract t (half_perm f));
+    //rewrite pts_to_Some h (half_perm f) as task_res_own h (half_perm f);
+    //assert (pts_to_Some h (half_perm f) ** pts_to_Some h (half_perm f));
+    //rewrite (pts_to_Some h (half_perm f)) as (task_res_own h (half_perm f));
+    share_tasks_res_own_general q f;
+    rewrite (task_res_own h (half_perm f) ** tasks_res_own q (half_perm f)) as (tasks_res_own l (half_perm f));
+    drop (tasks_res_own q (half_perm f));
+    //let x = Some?.v y;
+    //x
+    //unfold pts_to_Some h (half_perm f);
+    assert (pure (h._1 == t));
+    //with v. assert (pts_to h._1._2 #(half_perm f) v ** pure (Some? v));
+    rewrite (pts_to h._1._2 #(half_perm f) v ** pure (Some? v))
+      as (pts_to t._2 #(half_perm f) v ** pure (Some? v));
+    //rewrite (pts_to_Some h (half_perm f)) as (pts_to_Some_fract t (half_perm f));
+      //as (pts_to t._2 #(half_perm f) v ** pure (Some? v));
+    //intro_exists (fun v -> pts_to t._2 #(half_perm f) v ** pure (Some? v)) v;
+    fold pts_to_Some_fract t (half_perm f);
+    ()
   }
   else {
-    let x = get_Some_finished_aux_rec t pos q;
-    rewrite (task_res_own h ** tasks_res_own q) as (tasks_res_own l);
-    x
+    get_Some_finished_aux_rec t pos q f;
+    share_task_res_own h f;
+    rewrite (task_res_own h (half_perm f) ** tasks_res_own q (half_perm f))
+      as (tasks_res_own l (half_perm f));
+    drop (task_res_own h (half_perm f));
+    ()
   }
 }
 ```
+
+let recall_certificate_fract (#t: task_elem) (#pos: nat)
+           (r:ghost_mono_ref task_elem)
+           (v: mono_list task_elem)
+           (w:certificate r t pos)
+           (f: perm):
+ stt_ghost unit emp_inames
+                 (M.pts_to r f v)
+                 (fun _ -> M.pts_to r f v ** pure (task_in_queue t pos v))
+  = M.recall (task_in_queue t pos) r v w
+
+
 
 ```pulse
-ghost
-fn get_Some_finished'
-  (#t: task_elem) (#pos: nat)
-  (r:ghost_mono_ref task_elem)
+ghost fn
+proof_promise' (#t: task_elem) (#pos: nat)
+  (r: ghost_mono_ref task_elem)
   (w:certificate r t pos)
-requires small_inv r [] 0
-returns x: t._1
-ensures small_inv r [] 0
+requires deadline r
+ensures deadline r ** (exists_ (fun f -> (exists_ (fun v ->
+                          pts_to t._2 #f v ** pure (Some? v)))))
 {
-  unfold small_inv r [] 0;
-  with l. assert (pts_to_ghost_queue r (reveal l));
-  //with c. assert (pts_to c)
-  //let l : mono_list task_elem = l;
-  let ll = stt_ghost_reveal _ l;
-  if (L.length ll = 0) {
-    admit()
-  }
-  else {
-    admit()
-  }
-  (*
-  recall_certificate r l w;
-  assert (pure (task_in_queue t pos l));
-  assert (tasks_res_own l);
-  assert (pure (count_ongoing l = 0 /\ get_actual_queue l == []));
-  let x = get_Some_finished_aux t pos l;
-  fold small_inv r [] 0;
-  x
-  *)
+  unfold deadline r;
+  with f1 f2 l. assert (M.pts_to r f1 l ** tasks_res_own l f2
+    ** pure (count_ongoing l = 0 /\ get_actual_queue l == []));
+  recall_certificate_fract r l w f1;
+  get_Some_finished_aux t pos l f2;
+  assert (tasks_res_own l (half_perm f2) ** pts_to_Some_fract t (half_perm f2));
+  fold deadline r;
+  unfold (pts_to_Some_fract t (half_perm f2));
+  ()
 }
 ```
 
-let get_Some_finished = get_Some_finished'
+let proof_promise = proof_promise'
