share/steel/examples/pulse/parallel/GhostTaskQueue.fsti
@@ -3,75 +3,10 @@ module GhostTaskQueue
 module L = FStar.List.Tot.Base
 module P = FStar.Preorder
 
-// Mostly: Monotonic list of tasks with status
 type task_status = | Todo | Ongoing | Done
-// preorder: Todo -> Ongoing -> Done
-
 type task_with_status (a: Type) = a & task_status
 type mono_list (a: Type) = list (task_with_status a)
-
-// the list can only evolve according to this order
-// it imposes todo < ongoing < done, which we do not use
-val is_mono_suffix (#a: Type): P.preorder (mono_list a)
-
-val task_in_queue (#a: Type) (x: a) (pos:nat) (l: mono_list a): prop
-
-val task_in_queue_preorder (#a: Type)
-    (t: a) (pos: nat) (x y: mono_list a):
-Lemma (requires task_in_queue t pos x /\ is_mono_suffix x y)
-      (ensures task_in_queue t pos y)
-
-let rec count_ongoing #a (l: mono_list a): nat =
-match l with
-| [] -> 0
-| (_, s)::q -> (if s = Ongoing then 1 else 0) + count_ongoing q
-
-let get_actual_queue #a (l: mono_list a): list a =
-    L.map fst (L.filter (fun t -> Todo? (snd t)) l)
-
-// 1. enqueue: when spawning a new task
-// get a certificate for task_in_queue
-val enqueue_todo (#a: Type) (l: mono_list a) (t: a):
-(r:mono_list a{ get_actual_queue r == t::get_actual_queue l
-                /\ count_ongoing r == count_ongoing l
-                /\ r == (t, Todo)::l } &
-pos:nat{task_in_queue t pos r})
-
-val enqueue_preserves_order (#a: Type) (l: mono_list a) (t: a):
-Lemma (is_mono_suffix l (enqueue_todo l t)._1)
-
-// 2. pop: when a worker starts working on a task
-// it updates the task to "ongoing"
-val pop_todo_task (#a: Type) (l: mono_list a{~(get_actual_queue l == [])})
-: (t:a & r:mono_list a{ get_actual_queue l == t::get_actual_queue r
-                /\ count_ongoing r == count_ongoing l + 1 }
-  & pos:nat{task_in_queue t pos r})
-
-val pop_preserves_order (#a: Type) (l: mono_list a):
-Lemma (requires ~(get_actual_queue l == []))
-      (ensures is_mono_suffix l (pop_todo_task l)._2)
-
-(** 3. concluding the task: when the worker is done **)
-// a bit weird: Can we prove the task was not done before???
-// yes, because we have the permission?
-// maybe with 2/3 + 2/3 permissions
-val close_task (#a: Type)
-    (t: a)
-    (pos: nat)
-    (l: mono_list a{task_in_queue t pos l})
-  : (s:task_status{L.memP (t, s) l} & r:mono_list a{
-        s == Ongoing ==> (
-            get_actual_queue r == get_actual_queue l /\
-            count_ongoing r == count_ongoing l - 1)})
-
-val close_task_preserves_order (#a: Type)
-    (t: a) (pos: nat) (l: mono_list a{task_in_queue t pos l}):
-    Lemma (is_mono_suffix l (close_task t pos l)._2 )
-
-(** We connect the mono list with the actual queue and counter **)
-
-let pure_inv_queue #a (q: list a) (c: int) (l: mono_list a)
-= count_ongoing l = c /\ get_actual_queue l == q
+//val mono_list (a: Type): Type
 
 open Pulse.Lib.Pervasives
 
@@ -98,29 +33,41 @@ let task_elem: Type u#1 = (
 
 val ghost_mono_ref (a: Type u#1): Type0
 
-val pts_to_ghost_queue (#a: Type) (r: ghost_mono_ref a) (l: mono_list a): vprop
-
 val certificate (r:ghost_mono_ref task_elem) (t: task_elem) (pos: nat): Type0
 
+val deadline (r: ghost_mono_ref task_elem): vprop
+
+val duplicate_deadline (r: ghost_mono_ref task_elem):
+stt_ghost unit emp_inames (deadline r) (fun () -> deadline r ** deadline r)
+
 val small_inv (r: ghost_mono_ref task_elem) (q: list task_elem) (c: int): vprop 
+
+val extract_deadline (r: ghost_mono_ref task_elem):
+  stt_ghost unit emp_inames (small_inv r [] 0)
+    (fun () -> small_inv r [] 0 ** deadline r)
+
+let current_task r = (t:task_elem & pos:nat & certificate r t pos)
+let is_active #r (ct: current_task r): vprop =
+  (exists_ (fun v -> pts_to ct._1._2 #three_quart v))
 
 // 1. enqueue task
 val spawn_task_ghost
 (r: ghost_mono_ref task_elem)
-(q: list task_elem) (c: int) (t: task_elem):
-stt_ghost (erased (pos:nat & certificate r t pos)) emp_inames
-(small_inv r q c ** pts_to t._2 #three_quart None)
-(fun _ -> small_inv r (t::q) c)
+(q: list task_elem) (c: int) (t: task_elem)
+(ct: current_task r)
+: stt_ghost (erased (pos:nat & certificate r t pos)) emp_inames
+(small_inv r q c ** pts_to t._2 #three_quart None ** is_active ct)
+(fun _ -> small_inv r (t::q) c ** is_active ct)
 
 // 2. pop task todo
-// return certificate?
 val pop_task_ghost
 (r: ghost_mono_ref task_elem)
 (t: task_elem)
-(q: list task_elem) (c: int):
-stt_ghost (erased (pos:nat & certificate r t pos)) emp_inames
-(small_inv r (t::q) c)
-(fun _ -> small_inv r q (c + 1) ** pts_to t._2 #three_quart None)
+(q: list task_elem) (c: int)
+(ct: current_task r)
+: stt_ghost (erased (pos:nat & certificate r t pos)) emp_inames
+(small_inv r (t::q) c ** is_active ct)
+(fun _ -> small_inv r q (c + 1) ** pts_to t._2 #three_quart None ** is_active ct)
 
 val prove_task_ongoing
   (#t: task_elem)
@@ -128,9 +75,8 @@ val prove_task_ongoing
   (#v: option t._1)
   (r:ghost_mono_ref task_elem)
   (q: list task_elem) (c: int)
-  //(l: (l:mono_list task_elem{task_in_queue t pos l /\ L.length l >= 1})):
-  (w:certificate r t pos):
-stt_ghost unit emp_inames
+  (w:certificate r t pos)
+: stt_ghost unit emp_inames
 (small_inv r q c ** pts_to t._2 #three_quart v)
 (fun () -> small_inv r q c ** pts_to t._2 #three_quart v ** pure (c > 0))
 
@@ -140,6 +86,9 @@ val prove_ongoing_non_neg
 : stt_ghost unit emp_inames
 (small_inv r q c)
 (fun () -> small_inv r q c ** pure (c >= 0))
+
+let imp_vprop (b: bool) (p: vprop): vprop
+  = if b then p else emp
 
 // 3. conclude a task
 val conclude_task_ghost
@@ -151,22 +100,12 @@ val conclude_task_ghost
 (w: certificate r t pos):
 stt_ghost unit emp_inames
 (small_inv r q c ** pts_to t._2 #three_quart (Some x))
-(fun () -> small_inv r q (c - 1))
+(fun () -> small_inv r q (c - 1) ** imp_vprop (c = 1 && L.length q = 0) (deadline r))
 
-
-val recall_certificate (#t: task_elem) (#pos: nat)
-           (r:ghost_mono_ref task_elem)
-           (v: mono_list task_elem)
-           (w:certificate r t pos)
-  : //TODO: SteelAtomicU
- stt_ghost unit emp_inames
-                 (pts_to_ghost_queue r v)
-                 (fun _ -> pts_to_ghost_queue r v ** pure (task_in_queue t pos v))
-
-val get_Some_finished (#t: task_elem) (#pos: nat)
-  (r:ghost_mono_ref task_elem)
+val proof_promise (#t: task_elem) (#pos: nat)
+  (r: ghost_mono_ref task_elem)
   (w:certificate r t pos)
-: stt_ghost t._1 emp_inames
-(small_inv r [] 0)
-// that's the proof that it's finished
-(fun _ -> small_inv r [] 0)
+: stt_ghost unit emp_inames
+(deadline r)
+(fun () -> deadline r ** (exists_ (fun f -> (exists_ (fun v ->
+                          pts_to t._2 #f v ** pure (Some? v))))))
